spot/GC.SPOT.HeapExpansion.fst
@@ -9,7 +9,6 @@ open GC.Gen.MinorHeap
 open GC.Gen.Promote
 
 module MH = GC.Spec.MajorHeap
-module SeqMem = GC.Spec.SeqMemLemmas
 module SpecAlloc = GC.Spec.Allocator
 module SpecMajorAlloc = GC.Spec.MajorAllocator
 module CG = GC.Gen.CombinedGraph
@@ -98,23 +97,11 @@ let spot_ensure_capacity_expands_and_preserves_old_read
 
 let spot_chunked_classify_minor_field (ms: minor_state) (mh: MH.major_heap) (v: U64.t)
   : GTot (option CG.combined_vertex)
-  = let vo = to_minor_offset v in
-    if is_minor_addr vo && Seq.mem vo (minor_objects ms) then
-      Some (CG.MinorV vo)
-    else if is_val_addr v && Seq.mem (v <: obj_addr) (MH.major_objects mh) then
-      Some (CG.MajorV v)
-    else
-      None
+  = CG.chunked_classify_minor_field ms mh v
 
 let spot_chunked_classify_major_field (ms: minor_state) (mh: MH.major_heap) (v: U64.t)
   : GTot (option CG.combined_vertex)
-  = let vo = to_minor_offset v in
-    if is_minor_pointer vo && Seq.mem vo (minor_objects ms) then
-      Some (CG.MinorV vo)
-    else if is_val_addr v && Seq.mem (v <: obj_addr) (MH.major_objects mh) then
-      Some (CG.MajorV v)
-    else
-      None
+  = CG.chunked_classify_major_field ms mh v
 
 let spot_major_member_preserved_by_expansion
   (mh: MH.major_heap) (fresh: MH.heap_chunk) (fp: U64.t) (v: obj_addr)
@@ -126,27 +113,7 @@ let spot_major_member_preserved_by_expansion
           (MH.major_objects
             (SpecMajorAlloc.expand_major_heap mh fresh fp).major_out) ==
         Seq.mem v (MH.major_objects mh))
-  =
-  SpecMajorAlloc.expand_major_heap_objects mh fresh fp;
-  if Seq.mem v (MH.major_objects mh) then
-    SeqMem.seq_mem_cons_tail
-      (SpecMajorAlloc.fresh_chunk_object fresh)
-      v
-      (MH.major_objects mh)
-  else if
-    Seq.mem v
-      (MH.major_objects
-        (SpecMajorAlloc.expand_major_heap mh fresh fp).major_out)
-  then begin
-    SeqMem.seq_mem_cons_not_mem_implies_eq
-      (SpecMajorAlloc.fresh_chunk_object fresh)
-      v
-      (MH.major_objects mh);
-    SpecMajorAlloc.fresh_chunk_object_in_chunk fresh;
-    assert (v == SpecMajorAlloc.fresh_chunk_object fresh);
-    assert (MH.pointer_in_chunk fresh v);
-    assert False
-  end
+  = CG.chunked_major_member_preserved_by_expansion mh fresh fp v
 
 let spot_chunked_classify_minor_field_preserved_by_expansion
   (ms: minor_state) (mh: MH.major_heap) (fresh: MH.heap_chunk) (fp: U64.t)
@@ -158,12 +125,7 @@ let spot_chunked_classify_minor_field_preserved_by_expansion
         spot_chunked_classify_minor_field ms
           (SpecMajorAlloc.expand_major_heap mh fresh fp).major_out v ==
         spot_chunked_classify_minor_field ms mh v)
-  =
-  let vo = to_minor_offset v in
-  if is_minor_addr vo && Seq.mem vo (minor_objects ms) then ()
-  else if is_val_addr v then
-    spot_major_member_preserved_by_expansion mh fresh fp (v <: obj_addr)
-  else ()
+  = CG.chunked_classify_minor_field_preserved_by_expansion ms mh fresh fp v
 
 let spot_chunked_classify_major_field_preserved_by_expansion
   (ms: minor_state) (mh: MH.major_heap) (fresh: MH.heap_chunk) (fp: U64.t)
@@ -175,9 +137,4 @@ let spot_chunked_classify_major_field_preserved_by_expansion
         spot_chunked_classify_major_field ms
           (SpecMajorAlloc.expand_major_heap mh fresh fp).major_out v ==
         spot_chunked_classify_major_field ms mh v)
-  =
-  let vo = to_minor_offset v in
-  if is_minor_pointer vo && Seq.mem vo (minor_objects ms) then ()
-  else if is_val_addr v then
-    spot_major_member_preserved_by_expansion mh fresh fp (v <: obj_addr)
-  else ()
+  = CG.chunked_classify_major_field_preserved_by_expansion ms mh fresh fp v
